@@ -5,30 +5,30 @@ public import Roolean.QfBv.Assignment
 import Roolean.QfBv.Domain.Bitvector
 
 public def eval {v w} {α : Nat → Type} [Domain α]
-  (formula: Formula v w) (assignment: Assignment v α) : α w :=
+  (term: BvTerm v w) (assignment: Assignment v α) : α w :=
 
-  match formula with
-    | Formula.Constant constant => Domain.ofBitvector constant
+  match term with
+    | BvTerm.Constant constant => Domain.ofBitvector constant
 
-    | Formula.Variable index =>
+    | BvTerm.Variable index =>
       assignment.getElem index
 
-    | Formula.Unary inner op =>
+    | BvTerm.Unary inner op =>
       let inner := eval inner assignment
       Domain.uniOp inner op
 
-    | Formula.BinaryNormal left right op =>
+    | BvTerm.BinaryNormal left right op =>
       let left := eval left assignment
       let right := eval right assignment
       Domain.biNormal left right op
 
-    | Formula.BinaryReduction left right op =>
+    | BvTerm.BinaryReduction left right op =>
       let left := eval left assignment
       let right := eval right assignment
       Domain.biReduction left right op
 
 public theorem eval_sound {w v} {α : Nat → Type} [Domain α] [AbstractDomain α]
-  (f: Formula v w) (a: Assignment v α) (c: Assignment v Bitvector) (h: a.γ c)
+  (f: BvTerm v w) (a: Assignment v α) (c: Assignment v Bitvector) (h: a.γ c)
   : AbstractDomain.γ (eval f a) (eval f c) := by
   induction f
   {
@@ -61,12 +61,12 @@ public theorem eval_sound {w v} {α : Nat → Type} [Domain α] [AbstractDomain 
   }
 
 def eval3bv {v} {α : Nat → Type} [Domain α]
-  (formula: Formula v 1) (assignment: Assignment v α) : Option (Bitvector 1) :=
-  let result := eval formula assignment
+  (term: BvTerm v 1) (assignment: Assignment v α) : Option (Bitvector 1) :=
+  let result := eval term assignment
   Domain.toBitvector? result
 
 theorem eval3bv_sound {v} {α : Nat → Type} [Domain α] [AbstractDomain α]
-  (f: Formula v 1) (a: Assignment v α) (c: Assignment v Bitvector) (h: a.γ c)
+  (f: BvTerm v 1) (a: Assignment v α) (c: Assignment v Bitvector) (h: a.γ c)
   (r: Bitvector 1)
   : eval3bv f a = some r → eval f c = r := by
   simp[eval3bv]
@@ -79,13 +79,13 @@ theorem eval3bv_sound {v} {α : Nat → Type} [Domain α] [AbstractDomain α]
   simp[hToBvSound]
 
 public def eval3 {v} {α : Nat → Type} [Domain α]
-  (formula: Formula v 1) (assignment: Assignment v α) : Option Bool :=
-  match eval3bv formula assignment with
+  (term: BvTerm v 1) (assignment: Assignment v α) : Option Bool :=
+  match eval3bv term assignment with
     | some b => Bitvector.toBool b
     | none => none
 
 public theorem eval3_sound {v} {α : Nat → Type} [Domain α] [AbstractDomain α]
-  (f: Formula v 1) (a: Assignment v α) (c: Assignment v Bitvector) (h: a.γ c)
+  (f: BvTerm v 1) (a: Assignment v α) (c: Assignment v Bitvector) (h: a.γ c)
   (r: Bool)
   : eval3 f a = some r → (eval f c).toBool = r := by
   intro hEval
